ok
git-svn-id: svn://scm.gforge.inria.fr/svn/cfml@270 ba02c806-7d2b-4818-9a48-35b22e6bdc79

imper/Counter.ml
@@ -1,49 +1,14 @@
 
-
-
-let gensym () =
-   let x = ref 0 in
-   let f () = 
-      let n = !x in
-      x := n+1;
-      n in
+let make_counter () =
+   let r = ref 0 in
+   let f () = incr r; !r in
    f
 
-
 let rec iter f = function
-    [] -> ()
+  | [] -> ()
   | a::l -> f a; iter f l
 
+let ignore x = ()
 
-let test l = 
-  iter (fun f -> let i:int = f() in ()) l
-
-(*
-
-
-
-let test () =
-   let f = gensym() in
-   f() + f()
-*)
-
-
-
-(*  list de compteurs, à incrémenter un par un 
-
-let list_init n f =
-   let aux i =
-      if i = n then [] else (f i)::(aux (i+1)) in
-   aux 0
-
-let test_list n =
-   let syms = list_init n (fun _ => gensym()) in
-   for i = 0 to n do
-      let k = Random.int n in
-      let f = List.nth k syms in
-      ignore (f())
-   done;
-   let s = List.fold_left (fun acc f => acc + f()) 0 syms in
-   assert (s = syms) 
-
-*)
+let step_all (l:(unit->int)list) = 
+  iter (fun f -> ignore (f())) l
