imper/Counter_proof.v
@@ -1,20 +1,85 @@
 Set Implicit Arguments.
-Require Import LibCore CFPrim Counter_ml.
+Require Import CFLib Counter_ml.
 
-(*------------------------------------------------------------------*)
-(* code:
 
-let gensym () =
-   let x = ref 0 in
-   let f () = 
-      let n = !x in
-      x := n+1;
-      n in
-   f
+Notation "'LetFuncs' f1 ':=' Q1 'in' Q2" :=
+  (!F (fun H Q => forall f1, exists P1,
+     (Q1 -> P1 f1) /\ (P1 f1 -> Q2 H Q)))
+  (at level 69, f1 ident) : charac.
 
+Notation "'LetFun' f [ A1 ] x1 ':=' Q 'in' F" :=
+  (LetFunc f := (Body f [ A1 ] x1 => Q) in F)
+  (at level 69, f ident, x1 ident) : charac.
+  (* todo : other arities *)
+
+
+(********************************************************************)
+(* ** Counter function *)
+
+Definition CounterSpec I f :=
+  Spec f () |R>> forall m, R (I m) (\=(m+1) \*+ (I (m+1))).
+
+Definition Counter (n:int) (f:func) : hprop := 
+  Hexists I:int->hprop, I n \* [CounterSpec I f].
+
+Lemma Counter_apply : forall f n,
+  AppReturns f tt (f ~> Counter n) (\= (n+1) \*+ f ~> Counter (n+1)).
+Proof.
+  intros. hdata_simpl Counter. xextract as I Sf.
+  xapply_local (spec_elim_1 Sf tt n); hsimpl~.
+Qed.
+
+Lemma make_counter_spec : 
+  Specs make_counter () >> [] (~> Counter 0).
+Proof.
+  xcf. xapps. sets I: (fun n:int => r ~~> n).
+  xfun (CounterSpec I). xgo*. unfold I. hsimpl.
+  xret. hdata_simpl Counter. hsimpl~ I.
+Qed.
+
+
+
+(********************************************************************)
+(* ** List iterator *)
+
+Lemma iter_spec : forall A,
+  Spec iter (f:func) (l:list A) | R>>
+    forall H (Q:unit->hprop),
+    (forall (S:list A -> _ -> _ -> Prop),
+       is_local_1 S ->
+       (forall H Q, H ==> Q tt -> S nil H Q) ->
+       (forall H Q x l,
+          (localize H Q (fun (H:hprop) (Q:unit->hprop) => 
+             exists Q':unit->hprop,
+             app_1 f x H Q' /\ S l (Q' tt) Q) -> S (x::l) H Q)) ->
+      S l H Q) -> 
+   R H Q.
+Proof.
+  intros. xintros. intros f l H Q M.
+(*
+  specializes M (@app_2 Func (list A) unit iter f).  
+  forwards J: (iter_cf (K:= fun f' l' R => f' = f -> l' = l -> R H Q));
+   [ | | ]. skip. skip. lets: (spec_elim_2 J).
 *)
+ sets_eq S: (app_2 (A1:=val) (A2:=list A) (B:=unit) iter f). 
+ (*   specializes M S. *)
+  (* gen M. induction_wf IH: (@list_sub_wf A) l. intros M. apply M. *)
+  apply M; clear M H Q.
+  rewrite EQS. intros. xlocal.
+  intros H Q v.
+    rewrite EQS. eapply app_spec_2. xcf. intros. subst.
+    xmatch. xret~.
+  intros H Q x t J.
+    rewrite EQS. eapply app_spec_2. xcf. intros. subst.
+   xmatch.
+   applys local_weaken_formula J. clears H Q. intros H Q. intros (Q'&J1&J2). 
+   exists (Q' tt). split. skip. (* todo : fix apply J1. *) apply J2.
+Qed.
 
-(*------------------------------------------------------------------*)
+Hint Extern 1 (RegisterSpec iter) => Provide iter_spec.
+
+
+
 
 Definition counter_spec I f :=
   Spec f () |R>> forall n, R (I n) (\=n \*+ (I (n+1))).
