Makefile
@@ -102,8 +102,10 @@ VAC=\
 NEW=\
 	imper/MutableList_ml.v \
 	imper/Facto_ml.v \
+	imper/Counter_ml.v \
 	imper/Facto_proof.v \
-	imper/MutableList_proof.v 
+	imper/MutableList_proof.v \
+	imper/Counter_proof.v \
 
 IMP=\
 	CFHeaps.v \
@@ -116,12 +118,10 @@ IMP=\
 IMPER=\
 	imper/Landin_ml.v \
 	imper/Landin_proof.v \
-	imper/Counter_ml.v \
 	imper/TreeCopy_ml.v \
 	imper/Loops_ml.v \
 	imper/StrongUpdate_ml.v \
 	imper/InOut_ml.v \
-	imper/Counter_proof.v \
 	imper/Facto_proof.v \
 	imper/TreeCopy_proof.v \
 	imper/Loops_proof.v \
